Phi_System/IDE_CP.thy
@@ -1,5 +1,5 @@
 theory IDE_CP
-  imports IDE_CP_Reasoning3
+  imports IDE_CP_Reasoning3 IDE_CP_App2
 begin
 
 end
